comments, cleanup in join.v

join.v
@@ -8,6 +8,19 @@ Definition is_bool_val a :=
   | _ => false
   end.
 
+(* ------------------------------------------------------------ *)
+
+(* Parallel reduction: "a ⇒ b" the building block 
+   of our untyped, definitional equality.
+
+   This relation nondeterminstically does one-step
+   of beta-reduction in parallel throughout the term. 
+
+   Importantly, this relation is confluent (i.e. satisfies 
+   the diamond property), which leads to an easy proof of
+   confluence for its reflexive-transitive closure "⇒*".
+
+ *)
 Reserved Infix "⇒" (at level 60, right associativity).
 Inductive Par : tm -> tm -> Prop :=
 | P_Var i :
@@ -59,32 +72,270 @@ Inductive Par : tm -> tm -> Prop :=
   (* ---------- *)
   (tIf tFalse b0 c0) ⇒ c1
 | P_Bool :
+  (* ---------- *)
   tBool ⇒ tBool
 | P_Refl :
+  (* ---------- *)
   tRefl ⇒ tRefl
 | P_Eq a0 b0 A0 a1 b1 A1 :
   (a0 ⇒ a1) ->
   (b0 ⇒ b1) ->
   (A0 ⇒ A1) ->
+  (* ---------- *)
   (tEq a0 b0 A0) ⇒ (tEq a1 b1 A1)
 | P_J t0 a0 b0 p0 t1 a1 b1 p1 :
   (t0 ⇒ t1) ->
   (a0 ⇒ a1) ->
   (b0 ⇒ b1) ->
   (p0 ⇒ p1) ->
+  (* ---------- *)
   (tJ t0 a0 b0 p0) ⇒ (tJ t1 a1 b1 p1)
 | P_JRefl t0 a b t1 :
   (t0 ⇒ t1) ->
+  (* ---------- *)
   (tJ t0 a b tRefl) ⇒ t1
 where "A ⇒ B" := (Par A B).
 
 #[export]Hint Constructors Par : par.
 
+(* The reflexive, transitive closure of parallel reduction. *)
+
 Infix "⇒*" := (rtc Par) (at level 60, right associativity).
+
+(* Two types are Coherent when they reduce to a common type. *)
 
 Definition Coherent a0 a1 := (exists b, a0 ⇒* b /\ a1 ⇒* b).
 
-Lemma pars_pi_inv A B C (h : (tPi A B) ⇒* C) :
+(* ------------------------------------------------------------ *)
+
+(* Parallel reduction is reflexive *)
+
+Lemma Par_refl (a : tm) : a ⇒ a.
+Proof. elim : a; hauto lq:on ctrs:Par. Qed.
+
+(* Parallel reduction is contained in Coherent *)
+
+Lemma Par_Coherent a b :
+  (a ⇒ b) -> Coherent a b.
+Proof. hauto lq:on use:@rtc_once, @rtc_refl. Qed.
+
+
+(* ------------------------------------------------------------ *)
+
+(* A top-level beta-reduction is a parallel reduction *)
+Lemma P_AppAbs_cbn (a b b0 : tm) :
+  b0 = a [b..] ->
+  (tApp (tAbs a) b) ⇒ b0.
+Proof. hauto lq:on ctrs:Par use:Par_refl. Qed.
+
+(* convenience introduction form for P_AppAbs' *)
+Lemma P_AppAbs' a a0 b0 b b1 :
+  b = a0 [b1..] ->
+  (a ⇒ a0) ->
+  (b0 ⇒ b1) ->
+  (* ---------------------------- *)
+  (tApp (tAbs a) b0) ⇒ b.
+Proof. hauto lq:on use:P_AppAbs. Qed.
+
+
+(* ------------------------------------------------------------ *)
+
+(* Par (⇒), Pars (⇒* ), and ⇔ are closed under renaming *)
+
+Lemma Par_renaming a b (ξ : fin -> fin) :
+  (a ⇒ b) -> (a⟨ξ⟩ ⇒ b⟨ξ⟩).
+Proof.
+  move => h.
+  move : ξ.
+  elim : a b / h => /=; eauto with par.
+  - move => *.
+    apply : P_AppAbs'; eauto. by asimpl.
+Qed.
+
+Lemma Pars_renaming a b (ξ : fin -> fin) :
+  (a ⇒* b) -> (a⟨ξ⟩ ⇒* b⟨ξ⟩).
+Proof. induction 1; hauto lq:on ctrs:rtc use:Par_renaming. Qed.
+
+Lemma Coherent_renaming a b (ξ : fin -> fin) :
+  Coherent a b ->
+  Coherent a⟨ξ⟩ b⟨ξ⟩.
+Proof. hauto lq:on rew:off use:Pars_renaming. Qed.
+
+Local Lemma Par_morphing_lift (ξ0 ξ1 : fin -> tm)
+  (h : forall i, (ξ0 i ⇒ ξ1 i)) :
+  forall i, (up_tm_tm ξ0 i ⇒ up_tm_tm ξ1 i).
+Proof. case => [|i]; first by constructor. asimpl. by apply Par_renaming. Qed.
+
+(* ------------------------------------------------------------ *)
+
+(* Now we want to show all of the ways that these relations are closed 
+   under substitution. *)
+
+(* First, we extend the Par, Pars and Coherent relations to substitutions *)
+
+Definition Par_m (σ0 σ1 : fin -> tm) := (forall i, (σ0 i) ⇒ (σ1 i)).
+
+Infix "⇒ς"  := Par_m (at level 70, right associativity).
+Infix "⇒ς*" := (rtc Par_m) (at level 70, right associativity).
+
+Definition Coherent_m σ0 σ1 :=
+  exists σ, (σ0 ⇒ς* σ) /\ (σ1 ⇒ς* σ).
+
+(* Morphing lemmas *)
+(* TODO: make the names of these lemmas a little more meaningful? *)
+
+Lemma Par_morphing a b (σ0 σ1 : fin -> tm)
+  (h : σ0 ⇒ς σ1) :
+  (a ⇒ b) -> 
+  (a[σ0] ⇒ b[σ1]).
+Proof.
+  move => h0.
+  move : σ0 σ1 h.
+  elim : a b / h0; try solve [simpl; eauto with par].
+  - qauto db:par use: Par_morphing_lift.
+  - qauto l:on db:par use:Par_morphing_lift.
+  - move => a a0 b0 b1 h0 ih0 h1 ih1 σ0 σ h /=.
+    apply P_AppAbs' with (a0 := a0 [up_tm_tm σ]) (b1 := b1 [σ]).
+    by asimpl. hauto l:on unfold:Par_m use:Par_renaming inv:nat. eauto.
+  - hauto lq:on db:par use:Par_morphing_lift.
+Qed.
+
+
+Lemma Par_morphing_star a0 a1 (h : a0 ⇒* a1) (σ0 σ1 : fin -> tm) :
+  (σ0 ⇒ς σ1) ->
+  (a0[σ0] ⇒* a1 [σ1]).
+Proof.
+  induction h.
+  - move => h. apply @rtc_once. eauto using Par_morphing, Par_refl.
+  - move => h0.
+    apply : rtc_transitive; eauto.
+    apply @rtc_once.
+    sfirstorder use:Par_morphing, Par_refl.
+Qed.
+
+Lemma Coherent_morphing a0 a1 (h : Coherent a0 a1) (σ0 σ1 : fin -> tm) :
+  (σ0 ⇒ς σ1) ->
+  Coherent (a0[σ0]) (a1[σ1]).
+Proof.
+  hauto l:on use:Par_morphing_star, Par_refl, Par_Coherent unfold:Coherent, Par_m.
+Qed.
+
+Lemma Pars_morphing a b (σ0 σ1 : fin -> tm)
+  (h : σ0 ⇒ς* σ1) :
+  (a ⇒ b) ->
+  (a [σ0]) ⇒* (b[σ1]).
+Proof.
+  move : a b.
+  elim : σ0 σ1 / h.
+  - sfirstorder unfold:Par_m use:Par_morphing, @rtc_once, Par_refl.
+  - hauto lq:on unfold:Par_m use:Par_morphing, Par_refl ctrs:rtc.
+Qed.
+
+
+Lemma Pars_morphing_star a b (σ0 σ1 : fin -> tm)
+  (h : σ0 ⇒ς* σ1)
+  (h0 : a ⇒* b) :
+  (a [σ0] ⇒* b[σ1]).
+Proof.
+  elim : a b / h0.
+  - sfirstorder use:Pars_morphing, Par_refl.
+  - move => x y z /[swap] _.
+    move : Pars_morphing (rtc_refl Par_m σ0); repeat move /[apply].
+    apply rtc_transitive.
+Qed.
+
+Lemma Coherent_morphing_star a b σ0 σ1
+  (h : Coherent_m σ0 σ1)
+  (h0 : Coherent a b) :
+  Coherent (a[σ0]) (b[σ1]).
+Proof.
+  hauto q:on use:Pars_morphing_star unfold:Coherent.
+Qed.
+
+
+
+(* These two lemmas allow us to create substitutions
+   that are related by paralell reduction. *)
+
+Lemma good_Pars_morphing_ext a b σ0 σ1
+  (h : a ⇒* b) :
+  (σ0 ⇒ς* σ1) -> 
+  ((a .: σ0) ⇒ς* (b .: σ1)).
+Proof.
+  elim : a b /h.
+  - move => a.
+    move => h.
+    elim : σ0 σ1 / h; first by sfirstorder.
+    move => σ0 σ1 σ2 h h1.
+    apply rtc_transitive. apply rtc_once.
+    qauto l:on unfold:Par_m ctrs:rtc inv:nat use:Par_refl.
+  - move => x y z ha hb /[apply].
+    apply rtc_transitive. apply rtc_once.
+    hauto lq:on unfold:Par_m inv:nat use:Par_refl.
+Qed.
+
+Lemma good_Pars_morphing_ext2 a0 b0 a1 b1 σ0 σ1
+  (h : a0 ⇒* b0) (h1 : a1 ⇒*  b1) :
+  (σ0 ⇒ς* σ1) -> 
+  ((a0 .: (a1 .: σ0)) ⇒ς* (b0 .: (b1 .: σ1))).
+Proof. sfirstorder use:good_Pars_morphing_ext. Qed.
+
+
+(* The three relations are closed under substitution *)
+
+Lemma Par_subst a0 a1 (h : a0 ⇒ a1) (σ : fin -> tm) :
+  (a0[σ] ⇒ a1[σ]).
+Proof. hauto l:on unfold:Par_m use:Par_refl, Par_morphing. Qed.
+
+Lemma Par_subst_star a0 a1 (h : a0 ⇒* a1) (σ : fin -> tm) :
+  (a0 [σ]) ⇒* (a1 [σ]).
+Proof. hauto l:on use:Par_morphing_star, Par_refl unfold:Par_m. Qed.
+
+Lemma Coherent_subst_star a0 a1 (h : Coherent a0 a1) (σ : fin -> tm) :
+  Coherent (a0[σ]) (a1 [σ]).
+Proof. hauto lq:on use:Coherent_morphing, Par_refl unfold:Par_m. Qed.
+
+
+(* The relations are also closed under single substitution  *)
+
+(* TODO: is _cong the right name for these lemmas? *)
+
+Lemma Par_cong a0 a1 b0 b1 (h : a0 ⇒ a1) (h1 : b0 ⇒ b1) :
+  (a0 [b0..] ⇒ a1 [b1..]).
+Proof.
+  apply Par_morphing; auto.
+  case; auto.
+  sfirstorder use:Par_refl.
+Qed.
+
+
+Local Lemma Coherent_cong_helper : forall a0 c, (a0 ⇒* c) -> (a0.. ⇒ς* c..).
+Proof.
+  move => a0 c h2.
+  elim : a0 c / h2.
+    sfirstorder.
+    move => a b c ? ?.
+    apply rtc_transitive with (y := b..).
+    sauto lq:on unfold:Par_m inv:nat use:Par_refl use:good_Pars_morphing_ext. 
+Qed.
+
+Lemma Coherent_cong a0 a1 b0 b1
+  (h : Coherent a0 b0)
+  (h1 : Coherent a1 b1) :
+  Coherent (a1 [a0..]) (b1 [b0..]).
+Proof.
+  apply Coherent_morphing_star=>//.
+  sfirstorder use:Coherent_cong_helper.
+Qed.
+
+
+
+
+(* ------------------------------------------------------------ *)
+
+(* Inversion lemmas *)
+
+Lemma Pars_pi_inv A B C (h : (tPi A B) ⇒* C) :
   exists A0 B0, C = tPi A0 B0 /\ (A ⇒* A0) /\ (B ⇒* B0).
 Proof.
   move E : (tPi A B) h => T h.
@@ -92,7 +343,7 @@ Proof.
   elim : T C / h; hecrush inv:Par ctrs:Par, rtc.
 Qed.
 
-Lemma pars_eq_inv a b A C (h : (tEq a b A) ⇒* C) :
+Lemma Pars_eq_inv a b A C (h : (tEq a b A) ⇒* C) :
   exists a0 b0 A0, C = tEq a0 b0 A0 /\ a ⇒* a0 /\ b ⇒* b0 /\ A ⇒* A0.
 Proof.
   move E : (tEq a b A) h => T h.
@@ -102,12 +353,12 @@ Qed.
 
 Lemma Coherent_pi_inj A B A0 B0 (h : Coherent (tPi A B) (tPi A0 B0)) :
   Coherent A A0 /\ Coherent B B0.
-Proof. hauto q:on use:pars_pi_inv. Qed.
+Proof. hauto q:on use:Pars_pi_inv. Qed.
 
 Lemma Coherent_eq_inj a b A a0 b0 A0 (h : Coherent (tEq a b A) (tEq a0 b0 A0)) : Coherent a a0 /\ Coherent b b0 /\ Coherent A A0.
-Proof. hauto q:on use:pars_eq_inv. Qed.
+Proof. hauto q:on use:Pars_eq_inv. Qed.
 
-Lemma pars_univ_inv i A (h : (tUniv i) ⇒* A) :
+Lemma Pars_univ_inv i A (h : (tUniv i) ⇒* A) :
   A = tUniv i.
 Proof.
   move E : (tUniv i) h => A0 h.
@@ -116,15 +367,11 @@ Proof.
 Qed.
 
 Lemma Coherent_univ_inj i j (h : Coherent (tUniv i) (tUniv j)) : i = j.
-Proof. hauto lq:on rew:off inv:rtc use:pars_univ_inv. Qed.
+Proof. hauto lq:on rew:off inv:rtc use:Pars_univ_inv. Qed.
 
-Lemma Par_refl (a : tm) : a ⇒ a.
-Proof. elim : a; hauto lq:on ctrs:Par. Qed.
 
-Lemma P_AppAbs_cbn (a b b0 : tm) :
-  b0 = a [b..] ->
-  (tApp (tAbs a) b) ⇒ b0.
-Proof. hauto lq:on ctrs:Par use:Par_refl. Qed.
+(* ------------------------------------------------------------ *)
+
 
 Lemma P_IfTrue_star a b c :
   (a ⇒* tTrue) ->
@@ -170,189 +417,16 @@ Proof.
     apply P_J; sfirstorder use:Par_refl.
 Qed.
 
-Lemma P_AppAbs' a a0 b0 b b1 :
-  b = a0 [b1..] ->
-  (a ⇒ a0) ->
-  (b0 ⇒ b1) ->
-  (* ---------------------------- *)
-  (tApp (tAbs a) b0) ⇒ b.
-Proof. hauto lq:on use:P_AppAbs. Qed.
 
-Lemma par_renaming a b (ξ : fin -> fin) :
-  (a ⇒ b) ->
-  a⟨ξ⟩ ⇒ b⟨ξ⟩.
-  move => h.
-  move : ξ.
-  elim : a b / h => /=; eauto with par.
-  - move => *.
-    apply : P_AppAbs'; eauto. by asimpl.
-Qed.
-
-Lemma pars_renaming a b (ξ : fin -> fin) :
-  (a ⇒* b) ->
-  a⟨ξ⟩ ⇒* b⟨ξ⟩.
-Proof. induction 1; hauto lq:on ctrs:rtc use:par_renaming. Qed.
-
-Lemma Coherent_renaming a b (ξ : fin -> fin) :
-  Coherent a b ->
-  Coherent (a ⟨ ξ ⟩) (b ⟨ ξ ⟩).
-Proof. hauto lq:on rew:off use:pars_renaming. Qed.
-
-(* TODO: notation for up_tm_tm *)
-Lemma par_morphing_lift (ξ0 ξ1 : fin -> tm)
-  (h : forall i, (ξ0 i) ⇒ (ξ1 i)) :
-  forall i, (up_tm_tm ξ0 i) ⇒ (up_tm_tm ξ1 i).
-Proof.
-  case => [|i]; first by constructor.
-  asimpl.
-  by apply par_renaming.
-Qed.
-
-Lemma par_morphing a b (σ0 σ1 : fin -> tm)
-  (h : forall i, (σ0 i) ⇒ (σ1 i)) :
-  (a ⇒ b) ->
-  (a[σ0]) ⇒ (b[σ1]).
-Proof.
-  move => h0.
-  move : σ0 σ1 h.
-  elim : a b / h0; try solve [simpl; eauto with par].
-  - hauto lq:on db:par use:par_morphing_lift.
-  - hauto lq:on db:par use:par_morphing_lift.
-  - move => a a0 b0 b1 h0 ih0 h1 ih1 σ0 σ h /=.
-    apply P_AppAbs' with (a0 := a0 [up_tm_tm σ]) (b1 := b1 [σ]).
-    by asimpl. hauto l:on use:par_renaming inv:nat. eauto.
-  - hauto lq:on db:par use:par_morphing_lift.
-Qed.
-
-Inductive good_pars_morphing : (fin -> tm) -> (fin -> tm) -> Prop :=
-| good_pars_morphing_one σ :
-  good_pars_morphing σ σ
-| good_pars_morphing_cons σ0 σ1 σ2 :
-  (forall i, (σ0 i) ⇒ (σ1 i)) ->
-  good_pars_morphing σ1 σ2 ->
-  good_pars_morphing σ0 σ2.
-
-Lemma good_pars_morphing_ext a b σ0 σ1
-  (h : a ⇒* b) :
-  good_pars_morphing σ0 σ1 ->
-  good_pars_morphing (a .: σ0) (b .: σ1).
-Proof.
-  elim : a b /h.
-  - move => a.
-    move => h.
-    elim : σ0 σ1 / h; first by sfirstorder.
-    move => σ0 σ1 σ2 h h1.
-    apply good_pars_morphing_cons.
-    hauto lq:on inv:nat use:Par_refl.
-  - move => x y z ha hb /[apply].
-    apply : good_pars_morphing_cons.
-    hauto lq:on inv:nat use:Par_refl.
-Qed.
-
-Lemma good_pars_morphing_ext2 a0 b0 a1 b1 σ0 σ1
-  (h : a0 ⇒* b0) (h1 : a1 ⇒*  b1) :
-  good_pars_morphing σ0 σ1 ->
-  good_pars_morphing (a0 .: (a1 .: σ0)) (b0 .: (b1 .: σ1)).
-Proof. sfirstorder use:good_pars_morphing_ext. Qed.
-
-(* No idea how to induct on (forall i, Pars (σ0 i) (σ1 i) ) *)
-Lemma pars_morphing a b (σ0 σ1 : fin -> tm)
-  (h : good_pars_morphing σ0 σ1) :
-  (a ⇒ b) ->
-  (a [σ0]) ⇒* (b[σ1]).
-Proof.
-  move : a b.
-  elim : σ0 σ1 / h.
-  - sfirstorder use:par_morphing, @rtc_once, Par_refl.
-  - hauto lq:on use:par_morphing, Par_refl ctrs:rtc.
-Qed.
-
-Lemma pars_morphing_star a b (σ0 σ1 : fin -> tm)
-  (h : good_pars_morphing σ0 σ1)
-  (h0 : a ⇒* b) :
-  (a [σ0] ⇒* b[σ1]).
-Proof.
-  elim : a b / h0.
-  - sfirstorder use:pars_morphing, Par_refl.
-  - move => x y z /[swap] _.
-    move : pars_morphing (good_pars_morphing_one σ0); repeat move /[apply].
-    apply rtc_transitive.
-Qed.
-
-Definition good_coherent_morphing σ0 σ1 :=
-  exists σ, good_pars_morphing σ0 σ /\ good_pars_morphing σ1 σ.
-
-Lemma coherent_morphing_star a b σ0 σ1
-  (h : good_coherent_morphing σ0 σ1)
-  (h0 : Coherent a b) :
-  Coherent (a[σ0]) (b[σ1]).
-Proof.
-  hauto q:on use:pars_morphing_star unfold:Coherent.
-Qed.
-
-Lemma coherent_cong_helper : forall a0 c, (a0 ⇒* c) -> good_pars_morphing a0.. c.. .
-Proof.
-  move => a0 c h2.
-  elim : a0 c / h2.
-    sfirstorder.
-    move => a b c ? ?.
-    apply : good_pars_morphing_cons.
-    sauto lq:on inv:nat use:Par_refl. 
-Qed.
-
-Lemma coherent_cong a0 a1 b0 b1
-  (h : Coherent a0 b0)
-  (h1 : Coherent a1 b1) :
-  Coherent (a1 [a0..]) (b1 [b0..]).
-Proof.
-  apply coherent_morphing_star=>//.
-  sfirstorder use:coherent_cong_helper.
-Qed.
-
-Lemma par_cong a0 a1 b0 b1 (h : a0 ⇒ a1) (h1 : b0 ⇒ b1) :
-  (a0 [b0..] ⇒ a1 [b1..]).
-Proof.
-  apply par_morphing; auto.
-  case; auto.
-  sfirstorder use:Par_refl.
-Qed.
-
-Lemma par_subst a0 a1 (h : a0 ⇒ a1) (σ : fin -> tm) :
-  (a0[σ] ⇒ a1[σ]).
-Proof. hauto l:on use:Par_refl, par_morphing. Qed.
-
-Lemma par_morphing_star a0 a1 (h : a0 ⇒* a1) (σ0 σ1 : fin -> tm) :
-  (forall i, (σ0 i) ⇒ (σ1 i)) ->
-  (a0[σ0] ⇒* a1 [σ1]).
-Proof.
-  induction h.
-  - move => h. apply @rtc_once. eauto using par_morphing, Par_refl.
-  - move => h0.
-    apply : rtc_transitive; eauto.
-    apply @rtc_once.
-    sfirstorder use:par_morphing, Par_refl.
-Qed.
-
-Lemma Par_Coherent a b :
-  (a ⇒ b) -> Coherent a b.
-Proof. hauto lq:on use:@rtc_once, @rtc_refl. Qed.
-
-Lemma Coherent_morphing a0 a1 (h : Coherent a0 a1) (σ0 σ1 : fin -> tm) :
-  (forall i, (σ0 i) ⇒ (σ1 i)) ->
-  Coherent (a0[σ0]) (a1[σ1]).
-Proof.
-  hauto l:on use:par_morphing_star, Par_refl, Par_Coherent unfold:Coherent.
-Qed.
-
-Lemma par_subst_star a0 a1 (h : a0 ⇒* a1) (σ : fin -> tm) :
-  (a0 [σ]) ⇒* (a1 [σ]).
-Proof. hauto l:on use:par_morphing_star, Par_refl. Qed.
-
-Lemma Coherent_subst_star a0 a1 (h : Coherent a0 a1) (σ : fin -> tm) :
-  Coherent (a0[ σ]) (a1 [σ]).
-Proof. hauto lq:on use:Coherent_morphing, Par_refl. Qed.
+(* ------------------------------------------------------------ *)
 
 Derive Inversion Par_inv with (forall a b, a ⇒ b).
+
+(* ------------------------------------------------------------ *)
+
+(* We want to show that Coherent is an equivalence relation. But,
+   to show that it is transitive, we need to show that parallel 
+   reduction is confluent. *)
 
 (* Takahashi translation *)
 Function tstar (a : tm) :=
@@ -376,18 +450,20 @@ Function tstar (a : tm) :=
   | tJ t a b p => tJ (tstar t) (tstar a) (tstar b) (tstar p)
   end.
 
-Lemma par_triangle a : forall b, (a ⇒ b) -> (b ⇒ tstar a).
+Lemma Par_triangle a : forall b, (a ⇒ b) -> (b ⇒ tstar a).
 Proof.
-  apply tstar_ind; hauto lq:on inv:Par use:Par_refl,par_cong ctrs:Par.
+  apply tstar_ind; hauto lq:on inv:Par use:Par_refl,Par_cong ctrs:Par.
 Qed.
 
-Lemma par_confluent : diamond Par.
-Proof. hauto lq:on use:par_triangle unfold:diamond. Qed.
+Lemma Par_confluent : diamond Par.
+Proof. hauto lq:on use:Par_triangle unfold:diamond. Qed.
 
-Lemma pars_confluent : confluent Par.
+Lemma Pars_confluent : confluent Par.
 Proof.
-  sfirstorder use:par_confluent, @diamond_confluent.
+  sfirstorder use:Par_confluent, @diamond_confluent.
 Qed.
+
+(* Coherent is an equivalence relation *)
 
 Lemma Coherent_reflexive a :
   Coherent a a.
@@ -400,7 +476,7 @@ Proof. sfirstorder. Qed.
 Lemma Coherent_transitive a b c :
   Coherent a b -> Coherent b c -> Coherent a c.
 Proof.
-  have := pars_confluent.
+  have := Pars_confluent.
   move => h [z0 [? h0]] [z1 [h1 ?]].
   move /(_ b _ _ h0 h1) in h.
   case : h => z [*].
